code/experimental/P256/Hacl.Spec.ECDSAP256.Definition.fst
@@ -72,6 +72,76 @@ let wide_as_nat (h:mem) (e:widefelem) : GTot nat =
 
 
 noextract
+let scalar_as_nat (h: mem) (e: lbuffer uint8 (size 32)) = 
+    let s = as_seq h e in 
+    let s0 = s.[0] in
+    let s1 = s.[1] in
+    let s2 = s.[2] in
+    let s3 = s.[3] in
+    let s4 = s.[4] in
+    let s5 = s.[5] in
+    let s6 = s.[6] in
+    let s7 = s.[7] in
+    let s8 = s.[8] in
+    let s9 = s.[9] in
+    let s10 = s.[10] in
+    let s11 = s.[11] in
+    let s12 = s.[12] in
+    let s13 = s.[13] in
+    let s14 = s.[14] in
+    let s15 = s.[15] in
+    let s16 = s.[16] in
+    let s17 = s.[17] in
+    let s18 = s.[18] in
+    let s19 = s.[19] in
+    let s20 = s.[20] in
+    let s21 = s.[21] in
+    let s22 = s.[22] in
+    let s23 = s.[23] in
+    let s24 = s.[24] in
+    let s25 = s.[25] in
+    let s26 = s.[26] in
+    let s27 = s.[27] in
+    let s28 = s.[28] in
+    let s29 = s.[29] in
+    let s30 = s.[30] in
+    let s31 = s.[31] in
+    v s0 + v s1 * pow2 8 + v s2 * (pow2 (2 * 8)) + 
+    v s3 * (pow2 (3 * 8)) +
+    v s4 * (pow2 (4 * 8)) +
+    v s5 * (pow2 (5 * 8)) +
+    v s6 * (pow2 (6 * 8)) +
+    v s7 * (pow2 (7 * 8)) +
+    v s8 * (pow2 (8 * 8)) +
+    v s9 * (pow2 (9 * 8)) +
+    v s10 * (pow2 (10 * 8)) +
+    v s11 * (pow2 (11 * 8)) +
+    v s12 * (pow2 (12 * 8)) +
+    v s13 * (pow2 (13 * 8)) +
+    v s14 * (pow2 (14 * 8)) +
+    v s15 * (pow2 (15 * 8)) +
+    v s16 * (pow2 (16 * 8)) +
+    v s17 * (pow2 (17 * 8)) +
+    v s18 * (pow2 (18 * 8)) +
+    v s19 * (pow2 (19 * 8)) +
+    v s20 * (pow2 (20 * 8)) +
+    v s21 * (pow2 (21 * 8)) +
+    v s22 * (pow2 (22 * 8)) +
+    v s23 * (pow2 (23 * 8)) +
+    v s24 * (pow2 (24 * 8)) +
+    v s25 * (pow2 (25 * 8)) +
+    v s26 * (pow2 (26 * 8)) +
+    v s27 * (pow2 (27 * 8)) +
+    v s28 * (pow2 (28 * 8)) +
+    v s29 * (pow2 (29 * 8)) +
+    v s30 * (pow2 (30 * 8)) +
+    v s31 * (pow2 (31 * 8))
+
+    
+
+
+
+noextract
 let felem_seq_as_nat_8 (a: lseq uint64 8) : Tot nat = 
   let open FStar.Mul in 
   let a0 = Lib.Sequence.index a 0 in 
